proof/DDC/Language/SystemF2/TyJudge.v
@@ -1,18 +1,118 @@
 
-Require Import SubstTypeType.
-Require Import SubstTypeExp.
-Require Import TyJudge.
+Require Import DDC.Language.SystemF2.SubstTypeType.
+Require Export DDC.Language.SystemF2.Exp.
+Require Export DDC.Language.SystemF2.TyEnv.
+Require Export DDC.Language.SystemF2.KiJudge.
 
 
-(* Weakening Kind Env in TyJudge ************************************
+(* Type judgement assigns a type to an expression. *)
+Inductive TYPE : kienv -> tyenv -> exp -> ty -> Prop :=
+ | TYVar 
+   :  forall ix ke te t
+   ,  get ix te = Some t
+   -> KIND ke t KStar
+   -> TYPE ke te (XVar ix) t
+
+ | TYLam 
+   :  forall ke te x12 t11 t12
+   ,  KIND ke t11 KStar
+   -> TYPE ke (te :> t11)  x12            t12
+   -> TYPE ke  te         (XLam t11 x12) (tFun t11 t12)
+
+ | TYApp 
+   :  forall ke te x1 x2 t11 t12
+   ,  TYPE ke te x1 (tFun t11 t12) 
+   -> TYPE ke te x2 t11
+   -> TYPE ke te (XApp x1 x2) t12
+
+ | TYLAM
+   :  forall ke te x1 t1
+   ,  TYPE (ke :> KStar) (liftTE 0 te) x1        t1
+   -> TYPE ke            te           (XLAM x1) (TForall t1)
+
+ | TYAPP
+   :  forall ke te x1 t1 t2
+   ,  TYPE ke te x1 (TForall t1)
+   -> KIND ke t2 KStar
+   -> TYPE ke te (XAPP x1 t2) (substTT 0 t2 t1). 
+
+Hint Constructors TYPE.
+
+
+(* The type produced by a type judgement is well kinded *)
+Theorem type_kind
+ :  forall ke te x t
+ ,  TYPE ke te x t
+ -> KIND ke t KStar.
+Proof.
+ intros. gen ke te t.
+ induction x; intros; inverts H; eauto.
+ 
+ Case "XAPP".
+  apply IHx in H4. inverts H4.
+  eapply subst_type_type; eauto.
+
+ Case "XLam".
+  unfold tFun.
+  apply IHx in H6.
+  eapply KIApp.
+   eapply KIApp.
+   eauto. auto. auto.
+
+ Case "XApp".
+  apply IHx1 in H4.
+  apply IHx2 in H6.
+   unfold tFun in H4.
+    inverts H4.
+    inverts H2.
+    inverts H3.
+    auto.
+Qed.
+
+
+(* A well typed expression is well formed *)
+Theorem type_wfX
+ :  forall ke te x t
+ ,  TYPE ke te x t
+ -> wfX  ke te x.
+Proof.
+ intros. gen ke te t.
+ induction x; intros; simpl.
+
+ Case "XVar".
+  inverts H. eauto.
+
+ Case "XLAM".
+  inverts H.
+  apply IHx in H3. eauto.
+
+ Case "XAPP".
+  inverts H. 
+  lets D: IHx H4. split. 
+   auto. eapply kind_wfT. eauto.
+
+ Case "XLam".
+  inverts H.
+  apply IHx in H6.
+  apply kind_wfT in H4. auto.
+
+ Case "XApp".
+  inverts H.
+  apply IHx1 in H4. 
+  apply IHx2 in H6.
+   auto.
+Qed.
+Hint Resolve type_wfX.
+
+
+(* Weakening Kind Env in TyJudge.
    We can insert a new kind into the kind environment of a type
    judgement, provided we lift existing references to kinds higher
    than this in the stack over the new one.
 
    References to existing elements of the kind environment may
    appear in the type environment, expression, as well as the
-   resulting type -- so we must lift all of them.
- *)
+   resulting type -- so we must lift all of them. *)
 Lemma type_kienv_insert
  :  forall ix ke te x1 t1 k2
  ,  TYPE ke                 te             x1             t1
@@ -64,11 +164,10 @@ Proof.
 Qed.
 
 
-(* Weakening Type Env in TyJudge ************************************
+(* Weakening Type Env in TyJudge.
    We can insert a new type into the type environment of a type 
    judgement, provided we lift existing references to types higher
-   than this in the stack over the new one.
- *)
+   than this in the stack over the new one. *)
 Lemma type_tyenv_insert
  :  forall ke te ix x1 t1 t2
  ,  TYPE ke  te                x1            t1
@@ -105,66 +204,5 @@ Proof.
   destruct te; auto. rewrite H0.
   apply type_tyenv_insert. auto.
 Qed.
-
-
-(* Substitution of Values in Values preserves Typing ****************)
-Theorem subst_value_value_ix
- :  forall ix ke te x1 t1 x2 t2
- ,  get  te ix = Some t2
- -> TYPE ke te           x1 t1
- -> TYPE ke (drop ix te) x2 t2
- -> TYPE ke (drop ix te) (substXX ix x2 x1) t1.
-Proof.
- intros. gen ix ke te t1 x2 t2.
- induction x1; intros; inverts H0; simpl; eauto.
-
- Case "XVar".
-  fbreak_nat_compare.
-  SCase "n = ix".
-   rewrite H in H3. inverts H3. auto.
-
-  SCase "n < ix".
-   apply TYVar. 
-   rewrite <- H3. apply get_drop_above. auto. auto.
-
-  SCase "n > ix".
-   apply TYVar. auto.
-   rewrite <- H3.
-   destruct n.
-    burn.
-    simpl. nnat. apply get_drop_below. omega.
-    auto.
-
- Case "XLAM".
-  eapply (IHx1 ix) in H5.
-  apply TYLAM.
-   unfold liftTE. rewrite map_drop. eauto.
-   eapply get_map. eauto.
-   unfold liftTE. rewrite <- map_drop.
-    assert (map (liftTT 0) (drop ix te) = liftTE 0 (drop ix te)). 
-     unfold liftTE. auto. rewrite H0. clear H0.
-    apply type_kienv_weaken. auto.
-
- Case "XLam".
-  apply TYLam.
-   auto.
-   rewrite drop_rewind.
-   eapply IHx1; eauto.
-   simpl. apply type_tyenv_weaken. auto.
-Qed.
-
-
-Theorem subst_value_value
- :  forall ke te x1 t1 x2 t2
- ,  TYPE ke (te :> t2) x1 t1
- -> TYPE ke te x2 t2
- -> TYPE ke te (substXX 0 x2 x1) t1.
-Proof.
- intros.
- assert (te = drop 0 (te :> t2)). auto.
- rewrite H1. eapply subst_value_value_ix; eauto. eauto.
-Qed.
-
-
 
 
