proof/DDC/Language/SystemF2.v
@@ -1,0 +1,42 @@
+(* System-F2.
+   Like System-F, but with type-type application. *)
+
+(* Kinds and kind environemnts. *)
+Require Export DDC.Language.SystemF2.Ki.
+
+(* Types, well formed and closed, lifting and substitution lemmas. *)
+Require Export DDC.Language.SystemF2.Ty.
+
+(* Type environments, lifting and substitution lemmas. *)
+Require Export DDC.Language.SystemF2.TyEnv.
+
+(* Expressions, normal forms, lifting and substitution. *)
+Require Export DDC.Language.SystemF2.Exp.
+
+(* Kinds of types, weakening the kind environment. *)
+Require Export DDC.Language.SystemF2.KiJudge.
+
+(* Substitution of types in types preserves kinding. *)
+Require Export DDC.Language.SystemF2.SubstTypeType.
+
+(* Type Judgement. *)
+Require Export DDC.Language.SystemF2.TyJudge.
+
+(* Substitution of types in expressions preserves typing. *)
+Require Export DDC.Language.SystemF2.SubstTypeExp.
+
+(* Substitution of expressions in expressions preserves typing. *)
+Require Export DDC.Language.SystemF2.SubstExpExp.
+
+(* Small step evaluation. *)
+Require Export DDC.Language.SystemF2.Step.
+
+(* A well typed expression is either a value, or can take a step. *)
+Require Export DDC.Language.SystemF2.Progress.
+
+(* When an expression takes a step the results has the same type. *)
+Require Export DDC.Language.SystemF2.Preservation.
+
+(* Big step evaluation, and conversion to small steps. *)
+Require Export DDC.Language.SystemF2.Eval.
+
