proof/DDC/Language/SystemF2/Ki.v
@@ -1,0 +1,15 @@
+
+Require Export DDC.Base.
+
+(* Kinds *)
+Inductive ki : Type :=
+ | KStar   : ki
+ | KFun    : ki -> ki -> ki.
+Hint Constructors ki.
+
+
+(* Kind Environments *)
+Definition kienv := list ki.
+Hint Unfold kienv.
+
+
