proof/DDC/Language/SystemF2/SubstExpExp.v
@@ -1,0 +1,64 @@
+
+Require Import DDC.Language.SystemF2.SubstTypeType.
+Require Import DDC.Language.SystemF2.SubstTypeExp.
+Require Import DDC.Language.SystemF2.TyJudge.
+
+
+(* Substitution of exps in exps preserves typing *)
+Theorem subst_exp_exp_ix
+ :  forall ix ke te x1 t1 x2 t2
+ ,  get  ix te = Some t2
+ -> TYPE ke te           x1 t1
+ -> TYPE ke (delete ix te) x2 t2
+ -> TYPE ke (delete ix te) (substXX ix x2 x1) t1.
+Proof.
+ intros. gen ix ke te t1 x2 t2.
+ induction x1; intros; inverts H0; simpl; eauto.
+
+ Case "XVar".
+  fbreak_nat_compare.
+  SCase "n = ix".
+   rewrite H in H3. inverts H3. auto.
+
+  SCase "n < ix".
+   apply TYVar. 
+   rewrite <- H3. apply get_delete_above. auto. auto.
+
+  SCase "n > ix".
+   apply TYVar. auto.
+   rewrite <- H3.
+   destruct n.
+    burn.
+    simpl. nnat. apply get_delete_below. omega.
+    auto.
+
+ Case "XLAM".
+  eapply (IHx1 ix) in H5.
+  apply TYLAM.
+   unfold liftTE. rewrite map_delete. eauto.
+   eapply get_map. eauto.
+   unfold liftTE. rewrite <- map_delete.
+    assert (map (liftTT 0) (delete ix te) = liftTE 0 (delete ix te)). 
+     unfold liftTE. auto. rewrite H0. clear H0.
+    apply type_kienv_weaken. auto.
+
+ Case "XLam".
+  apply TYLam.
+   auto.
+   rewrite delete_rewind.
+   eapply IHx1; eauto.
+   simpl. apply type_tyenv_weaken. auto.
+Qed.
+
+
+Theorem subst_exp_exp
+ :  forall ke te x1 t1 x2 t2
+ ,  TYPE ke (te :> t2) x1 t1
+ -> TYPE ke te x2 t2
+ -> TYPE ke te (substXX 0 x2 x1) t1.
+Proof.
+ intros.
+ assert (te = delete 0 (te :> t2)). auto.
+ rewrite H1. eapply subst_exp_exp_ix; eauto. eauto.
+Qed.
+
