proof/DDC/Language/SystemF2/SubstTypeType.v
@@ -1,0 +1,54 @@
+
+Require Import DDC.Language.SystemF2.KiJudge.
+
+
+(* Substitution of types in types preserves kinding.
+   Must also subst new new type into types in env higher than ix
+   otherwise indices that reference subst type are broken, and 
+   the resulting type env would not be well formed *)
+Theorem subst_type_type_ix
+ :  forall ix ke t1 k1 t2 k2
+ ,  get ix ke = Some k2
+ -> KIND ke t1 k1
+ -> KIND (delete ix ke) t2 k2
+ -> KIND (delete ix ke) (substTT ix t2 t1) k1.
+Proof.
+ intros. gen ix ke t2 k1 k2.
+ induction t1; intros; simpl; inverts H0; eauto.
+
+ Case "TVar".
+  fbreak_nat_compare.
+  SCase "n = ix".
+   rewrite H in H4.
+   inverts H4. auto.
+
+  SCase "n < ix".
+   apply KIVar. rewrite <- H4.
+   apply get_delete_above; auto.
+
+  SCase "n > ix".
+   apply KIVar. rewrite <- H4.
+   destruct n.
+    burn.
+    simpl. nnat. apply get_delete_below. omega.
+
+ Case "TForall".
+  apply KIForall.
+  rewrite delete_rewind.
+  eapply IHt1; eauto.
+   apply kind_kienv_weaken. auto.
+Qed.
+
+
+Theorem subst_type_type
+ :  forall ke t1 k1 t2 k2
+ ,  KIND (ke :> k2) t1 k1
+ -> KIND ke         t2 k2
+ -> KIND ke (substTT 0 t2 t1) k1.
+Proof.
+ intros.
+ unfold substTT.
+ assert (ke = delete 0 (ke :> k2)). auto. rewrite H1.
+ eapply subst_type_type_ix; simpl; eauto.
+Qed.
+
