proof/Main.v
@@ -11,3 +11,6 @@ Require Import DDC.Language.SimplePCF.
 (* System-F. Like STLC, but with type abstraction and application. *)
 Require Import DDC.Language.SystemF.
 
+(* System-F2. Like System-F2 but with type-type application. *)
+Require Import DDC.Language.SystemF2.
+
